Поменял структуру тайпклассов в неравенствах.

Test.Float/Test.Float.Lemmas.Inequality.fst
@@ -16,32 +16,35 @@ let lt_lte a b : Lemma (requires a <. b) (ensures a <=. b) = ()
 
 type binop (a: Type) = a -> a -> bool
 
-class binrel (f: binop float) = {
+class binrel = {
+  op : binop float;
   intop: binop int;
   [@@@TC.no_method]
-  props : squash (forall a b. a `f` b <==> (base (a -. b) `intop` 0))
+  props : squash (forall a b. a `op` b <==> (base (a -. b) `intop` 0))
 }
 
-instance binrel_gt  : binrel ( >.) = { intop = ( >); props = () }
-instance binrel_lt  : binrel ( <.) = { intop = ( <); props = () }
-instance binrel_gte : binrel (>=.) = { intop = (>=); props = () }
-instance binrel_lte : binrel (<=.) = { intop = (<=); props = () }
+let (<?>) {| binrel |} a b = op a b
 
-let binrel_neg f {| binrel f |} a b : Lemma (f a b <==> f (~.b) (~.a)) =
+instance b_gt  : binrel = { op = ( >.); intop = ( >); props = () }
+instance b_lt  : binrel = { op = ( <.); intop = ( <); props = () }
+instance b_gte : binrel = { op = (>=.); intop = (>=); props = () }
+instance b_lte : binrel = { op = (<=.); intop = (<=); props = () }
+
+let binrel_neg {| binrel |} a b : Lemma (a <?> b <==> (~.b) <?> (~.a)) =
   distrib_neg_add b a;
   revert_sub a b
 
-let gt_neg  a b : Lemma ((a  >. b <==> ~.b  >. ~.a) /\ (a  >. b <==> ~.a  <. ~.b)) = binrel_neg ( >.) a b; gt_lt   ~.b ~.a
-let lt_neg  a b : Lemma ((a  <. b <==> ~.b  <. ~.a) /\ (a  <. b <==> ~.a  >. ~.b)) = binrel_neg ( <.) a b; gt_lt   ~.a ~.b
-let gte_neg a b : Lemma ((a >=. b <==> ~.b >=. ~.a) /\ (a >=. b <==> ~.a <=. ~.b)) = binrel_neg (>=.) a b; gte_lte ~.b ~.a
-let lte_neg a b : Lemma ((a <=. b <==> ~.b <=. ~.a) /\ (a <=. b <==> ~.a >=. ~.b)) = binrel_neg (<=.) a b; gte_lte ~.a ~.b
+let gt_neg  a b : Lemma ((a  >. b <==> ~.b  >. ~.a) /\ (a  >. b <==> ~.a  <. ~.b)) = binrel_neg #b_gt  a b; gt_lt   ~.b ~.a
+let lt_neg  a b : Lemma ((a  <. b <==> ~.b  <. ~.a) /\ (a  <. b <==> ~.a  >. ~.b)) = binrel_neg #b_lt  a b; gt_lt   ~.a ~.b
+let gte_neg a b : Lemma ((a >=. b <==> ~.b >=. ~.a) /\ (a >=. b <==> ~.a <=. ~.b)) = binrel_neg #b_gte a b; gte_lte ~.b ~.a
+let lte_neg a b : Lemma ((a <=. b <==> ~.b <=. ~.a) /\ (a <=. b <==> ~.a >=. ~.b)) = binrel_neg #b_lte a b; gte_lte ~.a ~.b
 
 
-let binrel_additive f {| binrel f |} a b c : Lemma
-  ((a `f` b <==> (a +. c) `f` (b +. c)) /\
-   (a `f` b <==> (a -. c) `f` (b -. c)))
+let binrel_additive {| binrel |} a b c : Lemma
+  ((a <?> b <==> (a +. c) <?> (b +. c)) /\
+   (a <?> b <==> (a -. c) <?> (b -. c)))
   =
-  let aux f {| binrel f |} a b c : Lemma (a `f` b <==> (a +. c) `f` (b +. c)) =
+  let aux {| binrel |} a b c : Lemma (a <?> b <==> (a +. c) <?> (b +. c)) =
     commut_add b c;
     assoc_add_right (a +. c) c b;
     assoc_add_right a c c;
@@ -50,13 +53,13 @@ let binrel_additive f {| binrel f |} a b c : Lemma
     add_zero a;
     assert ((a +. c) -. (b +. c) = a -. b)
   in
-  aux f a b c;
+  aux a b c;
   sub_is_add_neg a c;
   sub_is_add_neg b c;
-  aux f a b (~.c)
+  aux a b (~.c)
 
-let binrel_to_sub f {| binrel f |} a b : Lemma (a `f` b <==> (a -. b) `f` zero) =
-  binrel_additive f a b b;
+let binrel_to_sub {| binrel |} a b : Lemma (a <?> b <==> (a -. b) <?> zero) =
+  binrel_additive a b b;
   sub_self b
 
 let distrib_gt_zero a b : Lemma (requires a >. zero /\ b >=. zero) (ensures a +. b >. zero) =
@@ -81,30 +84,31 @@ let distrib_lt_zero a b : Lemma (requires a <. zero /\ b <=. zero) (ensures a +.
   assert (~.(a +. b) >. zero);
   lt_neg (a +. b) zero
 
-class weak_binrel (f: binop float) = {
-  op: binop float;
-  binrel_f : binrel f;
-  binrel_w: binrel op;
+class weak_pair = {
+  strong : binrel;
+  weak: binrel;
   [@@@TC.no_method]
   props : squash (
-    (forall a b. a `op` b <==> (a `f` b \/ a =. b)) /\
-    (forall (a: float{a `f` zero}) (b: float{b `op` zero}). (a +. b) `f` zero))
+    (forall a b. weak.op a b <==> (strong.op a b \/ a =. b)) /\
+    (forall (a: float{strong.op a zero}) (b: float{weak.op b zero}). strong.op (a +. b) zero)
+  )
 }
 
-instance weak_gt : weak_binrel (>.) = {
-  op = (>=.);
-  binrel_f = binrel_gt;
-  binrel_w = binrel_gte;
-  props = introduce forall (a: float{a >. zero}) (b: float{b >=. zero}). (a +. b) >. zero with distrib_gt_zero a b
+let (<??>) {| weak_pair |} a b = strong.op a b
+let (<?=>) {| weak_pair |} a b = weak.op a b
+
+instance weak_gt : weak_pair = {
+  strong = b_gt;
+  weak = b_gte;
+  props = introduce forall (a: float{a `b_gt.op` zero}) (b: float{b `b_gte.op` zero}). (a +. b) `b_gt.op` zero with distrib_gt_zero a b
 }
-instance weak_lt : weak_binrel (<.) = {
-  op = (<=.);
-  binrel_f = binrel_lt;
-  binrel_w = binrel_lte;
-  props = introduce forall (a: float{a <. zero}) (b: float{b <=. zero}). (a +. b) <. zero with distrib_lt_zero a b
+instance weak_lt : weak_pair = {
+  strong = b_lt;
+  weak = b_lte;
+  props = introduce forall (a: float{a `b_lt.op` zero}) (b: float{b `b_lte.op` zero}). (a +. b) `b_lt.op` zero with distrib_lt_zero a b
 }
 
-let binrel_commut f {| wb: weak_binrel f |} a b c : Lemma (requires a `f` b /\ b `wb.op` c) (ensures a `f` c) =
+let binrel_commut {| wp: weak_pair |} a b c : Lemma (requires a <??> b /\ b <?=> c) (ensures a <??> c) =
   add_zero a;
   sub_self (~.b);
   sub_is_add_neg (~.b) (~.b);
@@ -113,9 +117,9 @@ let binrel_commut f {| wb: weak_binrel f |} a b c : Lemma (requires a `f` b /\ b
   assoc_add_right (a +. ~.b) b c;
   sub_is_add_neg a b;
   assert (a -. c = (a -. b) +. (b -. c));
-  binrel_to_sub f #wb.binrel_f a b;
-  binrel_to_sub wb.op #wb.binrel_w b c;
-  binrel_to_sub f #wb.binrel_f a c
+  binrel_to_sub #wp.strong a b;
+  binrel_to_sub #wp.weak b c;
+  binrel_to_sub #wp.strong a c
 
-let commut_gt_gte a b c : Lemma (requires a >. b /\ b >=. c) (ensures a >. c) = binrel_commut (>.) a b c
-let commut_lt_lte a b c : Lemma (requires a <. b /\ b <=. c) (ensures a <. c) = binrel_commut (<.) a b c
+let commut_gt_gte a b c : Lemma (requires a >. b /\ b >=. c) (ensures a >. c) = binrel_commut #weak_gt a b c
+let commut_lt_lte a b c : Lemma (requires a <. b /\ b <=. c) (ensures a <. c) = binrel_commut #weak_lt a b c
